finish bvXor

src/BitBlastingSimple.v
@@ -1363,6 +1363,302 @@ Proof.
         by case: (interp_lit E ls1); case: (interp_lit E ls2); 
         rewrite /interp_lit !env_upd_eq .
 Qed .
+
+
+(* ===== bit_blast_xor ===== *)
+
+Definition bit_blast_xor1 (g: generator) (a1 a2: literal) : generator * cnf * literal :=
+  let (g', r) := gen g in
+  let cs := [[neg_lit r; a1; a2]; [neg_lit r; neg_lit a1; neg_lit a2]; 
+               [r; neg_lit a1; a2]; [r; a1; neg_lit a2]] in
+  (g', cs, r).
+
+Definition mk_env_xor1 E g a1 a2 : env * generator * cnf * literal :=
+  let (g', r) := gen g in
+  let E' := env_upd E (var_of_lit r)
+                    (xorb (interp_lit E a1) (interp_lit E a2)) in
+  let cs := [[neg_lit r; a1; a2]; [neg_lit r; neg_lit a1; neg_lit a2]; 
+               [r; neg_lit a1; a2]; [r; a1; neg_lit a2]] in
+  (E', g', cs, r).
+
+Fixpoint bit_blast_xor w (g: generator): w.-tuple literal -> w.-tuple literal -> generator * cnf * w.-tuple literal :=
+  if w is _.+1 then
+    fun ls1 ls2 =>
+      let (ls1_tl, ls1_hd) := eta_expand (splitlsb ls1) in
+      let (ls2_tl, ls2_hd) := eta_expand (splitlsb ls2) in
+      let '(g_hd, cs_hd, lrs_hd) := bit_blast_xor1 g ls1_hd ls2_hd in
+      let '(g_tl, cs_tl, lrs_tl) := bit_blast_xor g_hd ls1_tl ls2_tl in
+      (g_tl, cs_hd++cs_tl, cons_tuple lrs_hd lrs_tl)
+  else
+    fun _ _ =>
+      (g, [], [tuple]).
+
+Fixpoint mk_env_xor w (E : env) (g : generator) : w.-tuple literal -> w.-tuple literal -> env * generator * cnf * w.-tuple literal :=
+  if w is _.+1 then
+    fun ls1 ls2 =>
+      let (ls1_tl, ls1_hd) := eta_expand (splitlsb ls1) in
+      let (ls2_tl, ls2_hd) := eta_expand (splitlsb ls2) in
+      let '(E_hd, g_hd, cs_hd, lrs_hd) := mk_env_xor1 E g ls1_hd ls2_hd in
+      let '(E_tl, g_tl, cs_tl, lrs_tl) := mk_env_xor E_hd g_hd ls1_tl ls2_tl in
+      (E_tl, g_tl, cs_hd++cs_tl, cons_tuple lrs_hd lrs_tl)
+  else
+    fun _ _ =>
+      (E, g, [], [tuple]).
+
+Lemma bit_blast_xor1_correct :
+  forall g b1 b2 br E l1 l2 g' cs lr,
+    bit_blast_xor1 g l1 l2 = (g', cs, lr) ->
+    enc_bit E l1 b1 -> enc_bit E l2 b2 ->
+    interp_cnf E (add_prelude cs) ->
+    xorb b1 b2 = br ->
+    enc_bit E lr br.
+Proof.
+  move => g b1 b2 br E l1 l2 g' cs lr. rewrite /bit_blast_xor1 /enc_bit.
+  case => _ <- <-. move=> /eqP <- /eqP <- /andP /= [Htt Hcs] <-.
+  rewrite !interp_lit_neg_lit in Hcs. move: Hcs.
+  by case: (E g); case: (interp_lit E l1); case: (interp_lit E l2).
+Qed.      
+
+Lemma bit_blast_xor_correct :
+  forall w g (bs1 bs2 : BITS w) E ls1 ls2 g' cs lrs,
+    @bit_blast_xor w g ls1 ls2 = (g', cs, lrs) ->
+    enc_bits E ls1 bs1 ->
+    enc_bits E ls2 bs2 ->
+    interp_cnf E (add_prelude cs) ->
+    enc_bits E lrs (xorB bs1 bs2).
+Proof.
+  elim.
+  - done.
+  - move => n IH g. case/tupleP =>[ibs1_hd ibs1_tl]. case/tupleP =>[ibs2_hd ibs2_tl].
+    move => E. case/tupleP =>[ils1_hd ils1_tl]. case/tupleP =>[ils2_hd ils2_tl].
+    move => og cs. case/tupleP =>[ilrs1_hd ilrs1_tl].
+    rewrite /bit_blast_xor -/bit_blast_xor (lock bit_blast_xor)
+            (lock bit_blast_xor1) (lock interp_cnf)  /= !theadE !beheadCons -!lock.
+    case Hxor_hd: (bit_blast_xor1 g ils1_hd ils2_hd) =>[[g_hd cs_hd] lrs_hd].
+    case Hxor_tl: (bit_blast_xor g_hd ils1_tl ils2_tl) =>[[g_tl cs_tl] lrs_tl].
+    case => Hog <- Holrs_hd Holrs_tl => {cs}.
+    move => /andP [Henc1_hd Henc1_tl] /andP [Henc2_hd Hen2_tl] Hcnf.
+    rewrite add_prelude_append in Hcnf. move/andP: Hcnf => [Hcnf_hd Hcnf_tl].
+    rewrite /xorB. rewrite liftBinOpCons /=. rewrite /= !theadE !beheadCons.
+    apply/andP; split.
+    + rewrite -Holrs_hd.
+      exact: (bit_blast_xor1_correct Hxor_hd Henc1_hd Henc2_hd Hcnf_hd).
+    + apply: (IH g_hd ibs1_tl ibs2_tl E ils1_tl ils2_tl
+                 g_tl cs_tl ilrs1_tl _ Henc1_tl Hen2_tl Hcnf_tl).
+      rewrite Hxor_tl. apply: injective_projections => /=; first by reflexivity.
+      apply: val_inj. exact: Holrs_tl.
+Qed.
+
+Lemma mk_env_xor1_is_bit_blast_xor1 :
+  forall E g l1 l2 E' g' cs lr,
+    mk_env_xor1 E g l1 l2 = (E', g', cs, lr) ->
+    bit_blast_xor1 g l1 l2 = (g', cs, lr).
+Proof.
+  rewrite /mk_env_xor1 /bit_blast_xor1; intros;
+    dite_hyps; dcase_hyps; subst; reflexivity.
+Qed.
+
+Lemma mk_env_xor_is_bit_blast_xor :
+  forall w E g (ls1 ls2 : w.-tuple literal) E' g' cs lrs,
+    mk_env_xor E g ls1 ls2 = (E', g', cs, lrs) ->
+    bit_blast_xor g ls1 ls2 = (g', cs, lrs).
+Proof.
+  elim.
+  - move=> E g ls1 ls2 E' g' cs lrs /=. case=> _ <- <- <- //=.
+  - move=> n IHn E g. 
+    case/tupleP=> [ls1_hd ls1_tl]; case/tupleP=> [ls2_hd ls2_tl]. 
+    move=> E' g' cs; case/tupleP=> [lrs_hd lrs_tl].
+    rewrite /mk_env_xor -/mk_env_xor /bit_blast_xor -/bit_blast_xor.
+    rewrite (lock mk_env_xor1) (lock bit_blast_xor1) /= !theadE !beheadCons -!lock.
+    case Hhd : (mk_env_xor1 E g ls1_hd ls2_hd) => [[[E_hd g_hd] cs_hd] lsr_hd].
+    rewrite (mk_env_xor1_is_bit_blast_xor1 Hhd). 
+    case Htl : (mk_env_xor E_hd g_hd ls1_tl ls2_tl) => [[[E_tl g_tl] cs_tl] lsr_tl].
+    rewrite (IHn _ _ _ _ _ _ _ _ Htl).
+    case=> _ <- <- <- Hlsrtl. by rewrite -(tval_eq Hlsrtl). 
+Qed.
+
+Lemma mk_env_xor1_newer_gen :
+  forall E g l1 l2 E' g' cs lr,
+    mk_env_xor1 E g l1 l2 = (E', g', cs, lr) ->
+    (g <=? g')%positive.
+Proof.
+  rewrite /mk_env_xor1 => E g l1 l2 E' g' cs lr /=.
+  case=> _ <- _ _. exact: pos_leb_add_diag_r.
+Qed.
+
+Lemma mk_env_xor_newer_gen :
+  forall w E g (ls1 ls2 : w.-tuple literal) E' g' cs lrs,
+    mk_env_xor E g ls1 ls2 = (E', g', cs, lrs) ->
+    (g <=? g')%positive.
+Proof.
+  elim.
+  - move=> E g ls1 ls2 E' g' cs lrs. case=> _ <- _ _. exact: Pos.leb_refl.
+  - move=> n IHn E g.
+    case/tupleP => [ls1_hd ls1_tl]; case/tupleP => [ls2_hd ls2_tl]. 
+    move=> E' g' cs /tupleP [lrs_hd lrs_tl].
+    rewrite /mk_env_xor -/mk_env_xor. 
+    rewrite (lock mk_env_xor1) /= !theadE !beheadCons -!lock.
+    case Hhd : (mk_env_xor1 E g ls1_hd ls2_hd) => [[[E_hd g_hd] cs_hd] lsr_hd].
+    case Htl : (mk_env_xor E_hd g_hd ls1_tl ls2_tl) => [[[E_tl g_tl] cs_tl] lsr_tl].
+    case=> _ <- _ _ _. apply: pos_leb_trans.
+    - exact: (mk_env_xor1_newer_gen Hhd).
+    - exact: (IHn _ _ _ _ _ _ _ _ Htl).
+Qed.
+
+Lemma mk_env_xor1_newer_res :
+  forall E g l1 l2 E' g' cs lr,
+    mk_env_xor1 E g l1 l2 = (E', g', cs, lr) ->
+    newer_than_lit g l1 ->
+    newer_than_lit g l2 ->
+    newer_than_lit g' lr.
+Proof.
+  rewrite /mk_env_xor1 => E g l1 l2 E' g' cs lr /=.
+  case=> _ <- _ <-. move=> _ _; by apply newer_than_lit_add_diag_r.
+Qed.
+      
+Lemma mk_env_xor_newer_res :
+  forall w E g (ls1 ls2 : w.-tuple literal) E' g' cs lrs,
+    mk_env_xor E g ls1 ls2 = (E', g', cs, lrs) ->
+    newer_than_lits g ls1 ->
+    newer_than_lits g ls2 ->
+    newer_than_lits g' lrs.
+Proof.
+  elim.
+  - move=> E g ls1 ls2 E' g' cs lrs [] _ <- _ <- //=.
+  - move=> n IHn E g.
+    case/tupleP => [ls1_hd ls1_tl]; case/tupleP => [ls2_hd ls2_tl]. 
+    move=> E' g' cs /tupleP [lrs_hd lrs_tl].
+    rewrite /mk_env_xor -/mk_env_xor. 
+    rewrite (lock mk_env_xor1) /= !theadE !beheadCons -!lock.
+    case Hhd : (mk_env_xor1 E g ls1_hd ls2_hd) => [[[E_hd g_hd] cs_hd] lsr_hd].
+    case Htl : (mk_env_xor E_hd g_hd ls1_tl ls2_tl) => [[[E_tl g_tl] cs_tl] lsr_tl].
+    case=> _ <- _ <- <-. 
+    move/andP=> [Hgl1h Hgl1t] /andP [Hgl2h Hgl2t]. 
+    move : (mk_env_xor1_newer_res Hhd Hgl1h Hgl2h) => Hghlrh.
+    move : (mk_env_xor_newer_gen Htl) => Hghgt.
+    rewrite (newer_than_lit_le_newer Hghlrh Hghgt) /=.
+    move : (mk_env_xor1_newer_gen Hhd) => Hggh.
+    apply (IHn _ _ _ _ _ _ _ _ Htl).
+    + exact: (newer_than_lits_le_newer Hgl1t Hggh).
+    + exact: (newer_than_lits_le_newer Hgl2t Hggh).
+Qed.
+
+Lemma mk_env_xor1_newer_cnf :
+  forall E g l1 l2 E' g' cs lr,
+    mk_env_xor1 E g l1 l2 = (E', g', cs, lr) ->
+    newer_than_lit g l1 -> newer_than_lit g l2 ->
+    newer_than_cnf g' cs.
+Proof.
+  rewrite /mk_env_xor1 => E g l1 l2 E' g' cs lr /=.
+  case=> _ <- <- _. move=> Hgl1 Hgl2 /=. rewrite !newer_than_lit_neg. 
+  rewrite (newer_than_lit_add_diag_r (Pos g)).
+  rewrite (newer_than_lit_add_diag_r (Neg g)).
+  by rewrite !newer_than_lit_add_r. 
+Qed.
+
+Lemma mk_env_xor_newer_cnf :
+  forall w E g (ls1 ls2 : w.-tuple literal) E' g' cs lrs,
+    mk_env_xor E g ls1 ls2 = (E', g', cs, lrs) ->
+    newer_than_lits g ls1 -> newer_than_lits g ls2 ->
+    newer_than_cnf g' cs.
+Proof.
+  elim.
+  - move=> E g ls1 ls2 E' g' cs lrs [] _ <- <- _ //=.
+  - move=> n IHn E g.
+    case/tupleP => [ls1_hd ls1_tl]; case/tupleP => [ls2_hd ls2_tl]. 
+    move=> E' g' cs /tupleP [lrs_hd lrs_tl].
+    rewrite /mk_env_xor -/mk_env_xor. 
+    rewrite (lock mk_env_xor1) /= !theadE !beheadCons -!lock.
+    case Hhd : (mk_env_xor1 E g ls1_hd ls2_hd) => [[[E_hd g_hd] cs_hd] lsr_hd].
+    case Htl : (mk_env_xor E_hd g_hd ls1_tl ls2_tl) => [[[E_tl g_tl] cs_tl] lsr_tl].
+    case=> _ <- <- _ _ /=. 
+    move/andP=> [Hgl1h Hgl1t] /andP [Hgl2h Hgl2t]. 
+    rewrite newer_than_cnf_append.
+    move : (mk_env_xor1_newer_cnf Hhd Hgl1h Hgl2h) => Hghch.
+    move : (mk_env_xor_newer_gen Htl) => Hghgt.
+    rewrite (newer_than_cnf_le_newer Hghch Hghgt) /=.
+    move : (mk_env_xor1_newer_gen Hhd) => Hggh.
+    apply (IHn _ _ _ _ _ _ _ _ Htl).
+    + exact: (newer_than_lits_le_newer Hgl1t Hggh).
+    + exact: (newer_than_lits_le_newer Hgl2t Hggh).
+Qed.
+
+
+Lemma mk_env_xor1_preserve :
+  forall E g l1 l2 E' g' cs lr,
+    mk_env_xor1 E g l1 l2 = (E', g', cs, lr) ->
+    env_preserve E E' g.
+Proof.
+  rewrite /mk_env_xor1 => E g l1 l2 E' g' cs lr /=.
+  case=> <- _ _ _. by apply env_upd_eq_preserve.
+Qed.
+
+Lemma mk_env_xor_preserve :
+  forall w E g (ls1 ls2 : w.-tuple literal) E' g' cs lrs,
+    mk_env_xor E g ls1 ls2 = (E', g', cs, lrs) ->
+    env_preserve E E' g.
+Proof.
+  elim.
+  - move=> E g ls1 ls2 E' g' cs lrs [] <- _ _ _ //=.
+  - move=> n IHn E g.
+    case/tupleP => [ls1_hd ls1_tl]; case/tupleP => [ls2_hd ls2_tl]. 
+    move=> E' g' cs /tupleP [lrs_hd lrs_tl].
+    rewrite /mk_env_xor -/mk_env_xor. 
+    rewrite (lock mk_env_xor1) /= !theadE !beheadCons -!lock.
+    case Hhd : (mk_env_xor1 E g ls1_hd ls2_hd) => [[[E_hd g_hd] cs_hd] lsr_hd].
+    case Htl : (mk_env_xor E_hd g_hd ls1_tl ls2_tl) => [[[E_tl g_tl] cs_tl] lsr_tl].
+    case=> <- _ _ _ _ /=. 
+    move: (mk_env_xor1_preserve Hhd) => HpEEhg. 
+    move: (IHn _ _ _ _ _ _ _ _ Htl) => HpEhEtgh.
+    move: (mk_env_xor1_newer_gen Hhd) => Hggh.
+    move: (env_preserve_le HpEhEtgh Hggh). by apply env_preserve_trans.
+Qed.
+
+Lemma mk_env_xor1_sat :
+  forall E g l1 l2 E' g' cs lr,
+    mk_env_xor1 E g l1 l2 = (E', g', cs, lr) ->
+    newer_than_lit g l1 -> newer_than_lit g l2 ->
+    interp_cnf E' cs.
+Proof.
+  rewrite /mk_env_xor1 => E g l1 l2 E' g' cs lr /=.
+  case=> <- _ <- _ Hgl1 Hgl2. 
+  move: (newer_than_lit_neq Hgl1) (newer_than_lit_neq Hgl2) => Hngl1 Hngl2.
+  rewrite /= !env_upd_eq !interp_lit_neg_lit. 
+  rewrite (interp_lit_env_upd_neq _ _ Hngl1).
+  rewrite (interp_lit_env_upd_neq _ _ Hngl2).
+  by case (interp_lit E l1); case (interp_lit E l2).
+Qed.
+
+Lemma mk_env_xor_sat :
+  forall w E g (ls1 ls2 : w.-tuple literal) E' g' cs lrs,
+    mk_env_xor E g ls1 ls2 = (E', g', cs, lrs) ->
+    newer_than_lits g ls1 -> newer_than_lits g ls2 ->
+    interp_cnf E' cs.
+Proof.
+  elim.
+  - move=> E g ls1 ls2 E' g' cs lrs [] <- _ <- _ //=.
+  - move=> n IHn E g.
+    case/tupleP => [ls1_hd ls1_tl]; case/tupleP => [ls2_hd ls2_tl]. 
+    move=> E' g' cs /tupleP [lrs_hd lrs_tl].
+    rewrite /mk_env_xor -/mk_env_xor. 
+    rewrite (lock mk_env_xor1) /= !theadE !beheadCons -!lock.
+    case Hhd : (mk_env_xor1 E g ls1_hd ls2_hd) => [[[E_hd g_hd] cs_hd] lsr_hd].
+    case Htl : (mk_env_xor E_hd g_hd ls1_tl ls2_tl) => [[[E_tl g_tl] cs_tl] lsr_tl].
+    case=> <- _ <- _ _ /=. 
+    move/andP=> [Hgl1h Hgl1t] /andP [Hgl2h Hgl2t]. 
+    rewrite interp_cnf_append.
+    (* interp_cnf E_tl cs_hd *)
+    move: (mk_env_xor1_sat Hhd Hgl1h Hgl2h) => HiEhch.
+    move: (mk_env_xor_preserve Htl) => HpEhEtgh.
+    move: (mk_env_xor1_newer_cnf Hhd Hgl1h Hgl2h) => Hghch.
+    rewrite (env_preserve_cnf HpEhEtgh Hghch) HiEhch /=.
+    (* interp_cnf E_tl cs_tl *)
+    move: (mk_env_xor1_newer_gen Hhd) => Hggh.
+    apply (IHn _ _ _ _ _ _ _ _ Htl).
+    + exact: (newer_than_lits_le_newer Hgl1t Hggh).
+    + exact: (newer_than_lits_le_newer Hgl2t Hggh).
+Qed.
+
         
 (* ===== bit_blast_full_adder ===== *)
 
@@ -3892,7 +4188,11 @@ Fixpoint bit_blast_exp w (m : vm) (g : generator) (e : QFBV64.exp w) : vm * gene
                            let '(m2, g2, cs2, rs2) := bit_blast_exp m1 g1 e2 in
                            let '(g', cs, rs) := bit_blast_or g2 rs1 rs2 in
                            (m2, g', cs1 ++ cs2 ++ cs, rs)
-  | QFBV64.bvXor w e1 e2 => (m, g, [], copy w lit_tt) (* TODO *)
+  | QFBV64.bvXor w e1 e2 => 
+    let '(m1, g1, cs1, ls1) := bit_blast_exp m g e1 in
+    let '(m2, g2, cs2, ls2) := bit_blast_exp m1 g1 e2 in
+    let '(gr, csr, lsr) := bit_blast_xor g2 ls1 ls2 in
+    (m2, gr, cs1++cs2++csr, lsr)
   | QFBV64.bvNeg w e => (m, g, [], copy w lit_tt) (* TODO *)
   | QFBV64.bvAdd w e1 e2 => (m, g, [], copy w lit_tt) (* TODO *)
   | QFBV64.bvSub w e1 e2 => (m, g, [], copy w lit_tt) (* TODO *)
@@ -3980,7 +4280,11 @@ Fixpoint mk_env_exp w (m : vm) (s : QFBV64.State.t) (E : env) (g : generator) (e
     let '(m2, E2, g2, cs2, ls2) := mk_env_exp m1 s E1 g1 e2 in
     let '(E', g', cs, ls) := mk_env_or E2 g2 ls1 ls2 in
     (m2, E', g', cs1 ++ cs2 ++ cs, ls)
-  | QFBV64.bvXor w e1 e2 => (m, E, g, [], copy w lit_tt) (* TODO *)
+  | QFBV64.bvXor w e1 e2 => 
+    let '(m1, E1, g1, cs1, ls1) := mk_env_exp m s E g e1 in
+    let '(m2, E2, g2, cs2, ls2) := mk_env_exp m1 s E1 g1 e2 in
+    let '(Er, gr, csr, lsr) := mk_env_xor E2 g2 ls1 ls2 in
+    (m2, Er, gr, cs1++cs2++csr, lsr)
   | QFBV64.bvNeg w e => (m, E, g, [], copy w lit_tt) (* TODO *)
   | QFBV64.bvAdd w e1 e2 => (m, E, g, [], copy w lit_tt) (* TODO *)
   | QFBV64.bvSub w e1 e2 => (m, E, g, [], copy w lit_tt) (* TODO *)
@@ -4142,11 +4446,21 @@ Proof.
 Qed.
 
 Lemma bit_blast_exp_preserve_xor :
-  forall (w0 : nat) (e : QFBV64.exp w0) (e0 : QFBV64.exp w0) (m : vm) (g : generator)
-         (m' : vm) (g' : generator) (cs : cnf) (lrs : w0.-tuple literal),
-    bit_blast_exp m g (QFBV64.bvXor w0 e e0) = (m', g', cs, lrs) -> vm_preserve m m'.
+  forall (w : nat) (e1 : QFBV64.exp w),
+    (forall (m : vm) (g : generator)
+            (m' : vm) (g' : generator) (cs : cnf) (lrs : w.-tuple literal),
+        bit_blast_exp m g e1 = (m', g', cs, lrs) -> vm_preserve m m') ->
+    forall (e2 : QFBV64.exp w),
+      (forall (m : vm) (g : generator)
+              (m' : vm) (g' : generator) (cs : cnf) (lrs : w.-tuple literal),
+          bit_blast_exp m g e2 = (m', g', cs, lrs) -> vm_preserve m m') ->
+      forall (m : vm) (g : generator)
+             (m' : vm) (g' : generator) (cs : cnf) (lrs : w.-tuple literal),
+        bit_blast_exp m g (QFBV64.bvXor w e1 e2) = (m', g', cs, lrs) ->
+        vm_preserve m m'.
 Proof.
-Admitted.
+  auto_bit_blast_vm_preserve.
+Qed.
 
 Lemma bit_blast_exp_preserve_neg :
   forall (w0 : nat) (e : QFBV64.exp w0) (m : vm) (g : generator)
@@ -4515,7 +4829,9 @@ Proof.
   - move=> w e0 e1 .
     move: (bit_blast_exp_preserve _ e0) (bit_blast_exp_preserve _ e1) => IH0 IH1 .
     exact: (bit_blast_exp_preserve_or IH0 IH1) .
-  - exact: bit_blast_exp_preserve_xor.
+  - move=> w e1 e2.
+    move: (bit_blast_exp_preserve _ e1) (bit_blast_exp_preserve _ e2) => IH1 IH2.
+    exact: (bit_blast_exp_preserve_xor IH1 IH2).
   - exact: bit_blast_exp_preserve_neg.
   - exact: bit_blast_exp_preserve_add.
   - exact: bit_blast_exp_preserve_sub.
@@ -4693,15 +5009,41 @@ Proof.
 Qed .
 
 Lemma bit_blast_exp_xor :
-  forall (w0 : nat) (e e0 : QFBV64.exp w0) (m : vm) (g : generator)
-         (s : QFBV64.State.t) (E : env)
-         (m' : vm) (g' : generator) (cs : cnf) (lrs : w0.-tuple literal),
-    bit_blast_exp m g (QFBV64.bvXor w0 e e0) = (m', g', cs, lrs) ->
-    consistent m' E s ->
-    interp_cnf E (add_prelude cs) ->
-    enc_bits E lrs (QFBV64.eval_exp (QFBV64.bvXor w0 e e0) s).
+  forall (w : nat) (e1 : QFBV64.exp w),
+    (forall (m : vm) (g : generator) (s : QFBV64.State.t) (E : env)
+            (m' : vm) (g' : generator) (cs : cnf) (lrs : w.-tuple literal),
+        bit_blast_exp m g e1 = (m', g', cs, lrs) ->
+        consistent m' E s ->
+        interp_cnf E (add_prelude cs) ->
+        enc_bits E lrs (QFBV64.eval_exp e1 s)) ->
+    forall (e2 : QFBV64.exp w),
+      (forall (m : vm) (g : generator) (s : QFBV64.State.t) (E : env)
+              (m' : vm) (g' : generator) (cs : cnf) (lrs : w.-tuple literal),
+          bit_blast_exp m g e2 = (m', g', cs, lrs) ->
+          consistent m' E s ->
+          interp_cnf E (add_prelude cs) ->
+          enc_bits E lrs (QFBV64.eval_exp e2 s)) ->
+      forall (m : vm) (g : generator) (s : QFBV64.State.t) (E : env)
+             (m' : vm) (g' : generator)
+             (cs : cnf) (lrs : w.-tuple literal),
+        bit_blast_exp m g (QFBV64.bvXor w e1 e2) = (m', g', cs, lrs) ->
+        consistent m' E s ->
+        interp_cnf E (add_prelude cs) ->
+        enc_bits E lrs (QFBV64.eval_exp (QFBV64.bvXor w e1 e2) s).
 Proof.
-Admitted.
+  move=> w e1 IH1 e2 IH2 m g s E m' g' cs lrs.
+  rewrite (lock interp_cnf) /= -lock.
+  case He1 : (bit_blast_exp m g e1) => [[[m1 g1] cs1] ls1].
+  case He2 : (bit_blast_exp m1 g1 e2) => [[[m2 g2] cs2] ls2].
+  case Hr : (bit_blast_xor g2 ls1 ls2) => [[gr csr] lsr].
+  case=> <- _ <- <-. move=> Hcons2.
+  move: (vm_preserve_consistent (bit_blast_exp_preserve He2) Hcons2) => Hcons1.
+  move: (vm_preserve_consistent (bit_blast_exp_preserve He1) Hcons1) => Hcons0.
+  rewrite !add_prelude_append. move/andP=> [Hic1 /andP [Hic2 Hicr]].
+  apply: (bit_blast_xor_correct Hr _ _ Hicr).
+  - exact: (IH1 _ _ _ _ _ _ _ _ He1 Hcons1 Hic1).
+  - exact: (IH2 _ _ _ _ _ _ _ _ He2 Hcons2 Hic2).
+Qed.
 
 Lemma bit_blast_exp_neg :
   forall (w0 : nat) (e : QFBV64.exp w0) (m : vm) (g : generator)
@@ -5297,7 +5639,9 @@ Proof.
   - move => w e0 e1 .
     move: (bit_blast_exp_correct _ e0) (bit_blast_exp_correct _ e1) => IHe0 IHe1 .
     exact: (bit_blast_exp_or IHe0 IHe1) .
-  - exact: bit_blast_exp_xor.
+  - move=> w e1 e2.
+    move: (bit_blast_exp_correct _ e1) (bit_blast_exp_correct _ e2) => IH1 IH2.
+    exact: (bit_blast_exp_xor IH1 IH2).
   - exact: bit_blast_exp_neg.
   - exact: bit_blast_exp_add.
   - exact: bit_blast_exp_sub.
@@ -5440,13 +5784,32 @@ Proof.
 Qed .  
 
 Lemma mk_env_exp_is_bit_blast_exp_xor :
-  forall (w0 : nat) (e e0 : QFBV64.exp w0) (m : vm) (E : env)
-         (g : generator) (s : QFBV64.State.t) (m' : vm) (E' : env)
-         (g' : generator) (cs : cnf) (lrs : w0.-tuple literal),
-    mk_env_exp m s E g (QFBV64.bvXor w0 e e0) = (m', E', g', cs, lrs) ->
-    bit_blast_exp m g (QFBV64.bvXor w0 e e0) = (m', g', cs, lrs).
+  forall (w : nat) (e1 : QFBV64.exp w),
+    (forall (m : vm) (E : env) (g : generator) (s : QFBV64.State.t)
+            (m' : vm) (E' : env) (g' : generator) (cs : cnf)
+            (lrs : w.-tuple literal),
+        mk_env_exp m s E g e1 = (m', E', g', cs, lrs) ->
+        bit_blast_exp m g e1 = (m', g', cs, lrs)) ->
+    forall (e2 : QFBV64.exp w),
+      (forall (m : vm) (E : env) (g : generator) (s : QFBV64.State.t)
+              (m' : vm) (E' : env) (g' : generator) (cs : cnf)
+              (lrs : w.-tuple literal),
+          mk_env_exp m s E g e2 = (m', E', g', cs, lrs) ->
+          bit_blast_exp m g e2 = (m', g', cs, lrs)) ->
+      forall (m : vm) (E : env) (g : generator) (s : QFBV64.State.t)
+             (m' : vm) (E' : env) (g' : generator) (cs : cnf) 
+             (lrs : w.-tuple literal),
+        mk_env_exp m s E g (QFBV64.bvXor w e1 e2) = (m', E', g', cs, lrs) ->
+        bit_blast_exp m g (QFBV64.bvXor w e1 e2) = (m', g', cs, lrs).
 Proof.
-Admitted.
+  move=> w e1 IH1 e2 IH2 m E g s m' E' g' cs lrs /=.
+  case Hmke1 : (mk_env_exp m s E g e1) => [[[[m1 E1] g1] cs1] ls1].
+  case Hmke2 : (mk_env_exp m1 s E1 g1 e2) => [[[[m2 E2] g2] cs2] ls2].
+  case Hmkr : (mk_env_xor E2 g2 ls1 ls2) => [[[Er gr] csr] lsr].
+  case=> <- _ <- <- <-.
+  rewrite (IH1 _ _ _ _ _ _ _ _ _ Hmke1) (IH2 _ _ _ _ _ _ _ _ _ Hmke2).
+  by rewrite (mk_env_xor_is_bit_blast_xor Hmkr).
+Qed.
 
 Lemma mk_env_exp_is_bit_blast_exp_neg :
   forall (w0 : nat) (e : QFBV64.exp w0) (m : vm) (E : env)
@@ -5901,7 +6264,10 @@ Proof.
     move: (mk_env_exp_is_bit_blast_exp _ e0)
             (mk_env_exp_is_bit_blast_exp _ e1) => IHe0 IHe1 .
     exact: (mk_env_exp_is_bit_blast_exp_or IHe0 IHe1) .
-  - exact: mk_env_exp_is_bit_blast_exp_xor.
+  - move=> w e1 e2.
+    move: (mk_env_exp_is_bit_blast_exp _ e1) 
+          (mk_env_exp_is_bit_blast_exp _ e2) => IH1 IH2.
+    exact: (mk_env_exp_is_bit_blast_exp_xor IH1 IH2).
   - exact: mk_env_exp_is_bit_blast_exp_neg.
   - exact: mk_env_exp_is_bit_blast_exp_add.
   - exact: mk_env_exp_is_bit_blast_exp_sub.
@@ -6047,13 +6413,32 @@ Proof.
 Qed .
 
 Lemma mk_env_exp_newer_gen_xor :
-  forall (w0 : nat) (e e0 : QFBV64.exp w0) (m : vm) (s : QFBV64.State.t)
-         (E : env) (g : generator) (m' : vm) (E' : env) (g' : generator)
-         (cs : cnf) (lrs : w0.-tuple literal),
-    mk_env_exp m s E g (QFBV64.bvXor w0 e e0) = (m', E', g', cs, lrs) ->
-    (g <=? g')%positive.
+  forall (w : nat) (e1 : QFBV64.exp w),
+    (forall (m : vm) (s : QFBV64.State.t) (E : env) (g : generator)
+            (m' : vm) (E' : env) (g' : generator) (cs : cnf)
+            (lrs : w.-tuple literal),
+        mk_env_exp m s E g e1 = (m', E', g', cs, lrs) -> (g <=? g')%positive) ->
+    forall (e2 : QFBV64.exp w),
+      (forall (m : vm) (s : QFBV64.State.t) (E : env) (g : generator)
+              (m' : vm) (E' : env) (g' : generator) (cs : cnf)
+              (lrs : w.-tuple literal),
+          mk_env_exp m s E g e2 = (m', E', g', cs, lrs) -> (g <=? g')%positive) ->
+      forall (m : vm) (s : QFBV64.State.t) (E : env) (g : generator)
+             (m' : vm) (E' : env) (g' : generator) (cs : cnf) 
+             (lrs : w.-tuple literal),
+        mk_env_exp m s E g (QFBV64.bvXor w e1 e2) = (m', E', g', cs, lrs) ->
+        (g <=? g')%positive.
 Proof.
-Admitted.
+  move=> w e1 IH1 e2 IH2 m s E g m' E' g' cs lrs /=.
+  case Hmke1 : (mk_env_exp m s E g e1) => [[[[m1 E1] g1] cs1] ls1].
+  case Hmke2 : (mk_env_exp m1 s E1 g1 e2) => [[[[m2 E2] g2] cs2] ls2].
+  case Hmkr : (mk_env_xor E2 g2 ls1 ls2) => [[[Er gr] csr] lsr].
+  case=> _ _ <- _ _.
+  move: (IH1 _ _ _ _ _ _ _ _ _ Hmke1) => Hg0g1.
+  move: (IH2 _ _ _ _ _ _ _ _ _ Hmke2) => Hg1g2.
+  move: (mk_env_xor_newer_gen Hmkr) => Hg2gr.
+  apply: (pos_leb_trans Hg0g1). apply (pos_leb_trans Hg1g2). done.
+Qed.
 
 Lemma mk_env_exp_newer_gen_neg :
   forall (w0 : nat) (e : QFBV64.exp w0) (m : vm) (s : QFBV64.State.t)
@@ -6513,7 +6898,9 @@ Proof.
   - move => w e0 e1 .
     move: (mk_env_exp_newer_gen _ e0) (mk_env_exp_newer_gen _ e1) => IHe0 IHe1 .
     exact: (mk_env_exp_newer_gen_or IHe0 IHe1) .
-  - exact: mk_env_exp_newer_gen_xor.
+  - move=> w e1 e2.
+    move: (mk_env_exp_newer_gen _ e1) (mk_env_exp_newer_gen _ e2) => IH1 IH2.
+    exact: (mk_env_exp_newer_gen_xor IH1 IH2).
   - exact: mk_env_exp_newer_gen_neg.
   - exact: mk_env_exp_newer_gen_add.
   - exact: mk_env_exp_newer_gen_sub.
@@ -6666,13 +7053,34 @@ Proof.
 Qed .
 
 Lemma mk_env_exp_newer_vm_xor :
-  forall (w0 : nat) (e e0 : QFBV64.exp w0) (m : vm) (s : QFBV64.State.t)
-         (E : env) (g : generator) (m' : vm) (E' : env) (g' : generator)
-         (cs : cnf) (lrs : w0.-tuple literal),
-    mk_env_exp m s E g (QFBV64.bvXor w0 e e0) = (m', E', g', cs, lrs) ->
-    newer_than_vm g m -> newer_than_vm g' m'.
+  forall (w : nat) (e1 : QFBV64.exp w),
+    (forall (m : vm) (s : QFBV64.State.t) (E : env) (g : generator)
+            (m' : vm) (E' : env) (g' : generator) (cs : cnf)
+            (lrs : w.-tuple literal),
+        mk_env_exp m s E g e1 = (m', E', g', cs, lrs) ->
+        newer_than_vm g m -> newer_than_vm g' m') ->
+    forall (e2 : QFBV64.exp w),
+      (forall (m : vm) (s : QFBV64.State.t) (E : env) (g : generator)
+              (m' : vm) (E' : env) (g' : generator) (cs : cnf)
+              (lrs : w.-tuple literal),
+          mk_env_exp m s E g e2 = (m', E', g', cs, lrs) ->
+          newer_than_vm g m -> newer_than_vm g' m') ->
+      forall (m : vm) (s : QFBV64.State.t) (E : env) (g : generator)
+             (m' : vm) (E' : env) (g' : generator) (cs : cnf) 
+             (lrs : w.-tuple literal),
+        mk_env_exp m s E g (QFBV64.bvXor w e1 e2) = (m', E', g', cs, lrs) ->
+        newer_than_vm g m -> newer_than_vm g' m'.
 Proof.
-Admitted.
+  move=> w e1 IH1 e2 IH2 m s E g m' E' g' cs lrs /=.
+  case Hmke1 : (mk_env_exp m s E g e1) => [[[[m1 E1] g1] cs1] ls1].
+  case Hmke2 : (mk_env_exp m1 s E1 g1 e2) => [[[[m2 E2] g2] cs2] ls2].
+  case Hmkr : (mk_env_xor E2 g2 ls1 ls2) => [[[Er gr] csr] lsr].
+  case=> <- _ <- _ _ Hg0m0.
+  move: (IH1 _ _ _ _ _ _ _ _ _ Hmke1 Hg0m0) => Hg1m1.
+  move: (IH2 _ _ _ _ _ _ _ _ _ Hmke2 Hg1m1) => Hg2m2.
+  move: (mk_env_xor_newer_gen Hmkr) => Hg2gr.
+  exact: (newer_than_vm_le_newer Hg2m2 Hg2gr).
+Qed.
 
 Lemma mk_env_exp_newer_vm_neg :
   forall (w0 : nat) (e : QFBV64.exp w0) (m : vm) (s : QFBV64.State.t)
@@ -7139,7 +7547,9 @@ Proof.
   - move => w e0 e1 .
     move: (mk_env_exp_newer_vm _ e0) (mk_env_exp_newer_vm _ e1) => IHe0 IHe1 .
     exact: (mk_env_exp_newer_vm_or IHe0 IHe1) .
-  - exact: mk_env_exp_newer_vm_xor.
+  - move=> w e1 e2.
+    move: (mk_env_exp_newer_vm _ e1) (mk_env_exp_newer_vm _ e2) => IH1 IH2.
+    exact: (mk_env_exp_newer_vm_xor IH1 IH2).
   - exact: mk_env_exp_newer_vm_neg.
   - exact: mk_env_exp_newer_vm_add.
   - exact: mk_env_exp_newer_vm_sub.
@@ -7306,13 +7716,43 @@ Proof.
 Qed .
 
 Lemma mk_env_exp_newer_res_xor :
-  forall (w0 : nat) (e e0 : QFBV64.exp w0) (m : vm) (s : QFBV64.State.t)
-         (E : env) (g : generator) (m' : vm) (E' : env) (g' : generator)
-         (cs : cnf) (lrs : w0.-tuple literal),
-    mk_env_exp m s E g (QFBV64.bvXor w0 e e0) = (m', E', g', cs, lrs) ->
-    newer_than_vm g m -> newer_than_lit g lit_tt -> newer_than_lits g' lrs.
+  forall (w : nat) (e1 : QFBV64.exp w),
+    (forall (m : vm) (s : QFBV64.State.t) (E : env) (g : generator) 
+            (m' : vm) (E' : env) (g' : generator)
+            (cs : cnf) (lrs : w.-tuple literal),
+        mk_env_exp m s E g e1 = (m', E', g', cs, lrs) ->
+        newer_than_vm g m -> newer_than_lit g lit_tt -> 
+        newer_than_lits g' lrs) ->
+    forall (e2 : QFBV64.exp w),
+      (forall (m : vm) (s : QFBV64.State.t) (E : env) (g : generator) 
+              (m' : vm) (E' : env) (g' : generator)
+              (cs : cnf) (lrs : w.-tuple literal),
+          mk_env_exp m s E g e2 = (m', E', g', cs, lrs) ->
+          newer_than_vm g m -> newer_than_lit g lit_tt -> 
+          newer_than_lits g' lrs) ->
+      forall (m : vm) (s : QFBV64.State.t) (E : env) (g : generator) 
+             (m' : vm) (E' : env) (g' : generator)
+             (cs : cnf) (lrs : w.-tuple literal),
+        mk_env_exp m s E g (QFBV64.bvXor w e1 e2) = (m', E', g', cs, lrs) ->
+        newer_than_vm g m -> newer_than_lit g lit_tt -> newer_than_lits g' lrs.
 Proof.
-Admitted.
+  move=> w e1 IH1 e2 IH2 m s E g m' E' g' cs lrs /=.
+  case Hmke1 : (mk_env_exp m s E g e1) => [[[[m1 E1] g1] cs1] ls1].
+  case Hmke2 : (mk_env_exp m1 s E1 g1 e2) => [[[[m2 E2] g2] cs2] ls2].
+  case Hmkr : (mk_env_xor E2 g2 ls1 ls2) => [[[Er gr] csr] lsr].
+  case=> _ _ <- _ <- Hgm Hgt.
+  move: (IH1 _ _ _ _ _ _ _ _ _ Hmke1 Hgm Hgt) => Hg1l1.
+  (* newer_than_lits g2 ls2 *)
+  move: (mk_env_exp_newer_vm Hmke1 Hgm) => Hg1m1.
+  move: (mk_env_exp_newer_gen Hmke1) => Hgg1.
+  move: (newer_than_lit_le_newer Hgt Hgg1) => Hg1t.
+  move: (IH2 _ _ _ _ _ _ _ _ _ Hmke2 Hg1m1 Hg1t) => Hg2l2.
+  (* newer_than_lits g2 ls1 *)
+  move: (mk_env_exp_newer_gen Hmke2) => Hg1g2.
+  move: (newer_than_lits_le_newer Hg1l1 Hg1g2) => Hg2l1.
+  (* now mk_env_and_newer_res is available *)
+  exact: (mk_env_xor_newer_res Hmkr Hg2l1 Hg2l2).
+Qed.
 
 Lemma mk_env_exp_newer_res_neg :
   forall (w0 : nat) (e : QFBV64.exp w0) (m : vm) (s : QFBV64.State.t)
@@ -7728,7 +8168,9 @@ Proof.
   - intros . move: (mk_env_exp_newer_res _ e) => IHe .
     move: (mk_env_exp_newer_res _ e0) => IHe0 .
     exact: (mk_env_exp_newer_res_or IHe IHe0 H H0 H1) .
-  - exact: mk_env_exp_newer_res_xor.
+  - move=> w0 e1 e2.
+    move: (mk_env_exp_newer_res _ e1) (mk_env_exp_newer_res _ e2) => IH1 IH2.
+    exact: (mk_env_exp_newer_res_xor IH1 IH2).
   - exact: mk_env_exp_newer_res_neg.
   - exact: mk_env_exp_newer_res_add.
   - exact: mk_env_exp_newer_res_sub.
@@ -7913,15 +8355,55 @@ Proof.
 Qed.
 
 Lemma mk_env_exp_newer_cnf_xor :
-  forall (w0 : nat) (e e0 : QFBV64.exp w0) (m : vm) (s : QFBV64.State.t)
-         (E : env) (g : generator) (m' : vm) (E' : env) (g' : generator)
-         (cs : cnf) (lrs : w0.-tuple literal),
-    mk_env_exp m s E g (QFBV64.bvXor w0 e e0) = (m', E', g', cs, lrs) ->
-    newer_than_vm g m ->
-    newer_than_lit g lit_tt ->
-    newer_than_cnf g' cs.
+  forall (w : nat) (e1 : QFBV64.exp w),
+    (forall (m : vm) (s : QFBV64.State.t) (E : env) (g : generator)
+            (m' : vm) (E' : env) (g' : generator) (cs : cnf)
+            (lrs : w.-tuple literal),
+        mk_env_exp m s E g e1 = (m', E', g', cs, lrs) ->
+        newer_than_vm g m ->
+        newer_than_lit g lit_tt ->
+        newer_than_cnf g' cs) ->
+    forall (e2 : QFBV64.exp w),
+      (forall (m : vm) (s : QFBV64.State.t) (E : env) (g : generator)
+              (m' : vm) (E' : env) (g' : generator) (cs : cnf)
+              (lrs : w.-tuple literal),
+          mk_env_exp m s E g e2 = (m', E', g', cs, lrs) ->
+          newer_than_vm g m ->
+          newer_than_lit g lit_tt ->
+          newer_than_cnf g' cs) ->
+      forall (m : vm) (s : QFBV64.State.t) (E : env) (g : generator)
+             (m' : vm) (E' : env) (g' : generator) (cs : cnf) 
+             (lrs : w.-tuple literal),
+        mk_env_exp m s E g (QFBV64.bvXor w e1 e2) = (m', E', g', cs, lrs) ->
+        newer_than_vm g m ->
+        newer_than_lit g lit_tt ->
+        newer_than_cnf g' cs.
 Proof.
-Admitted.
+  move=> w e1 IH1 e2 IH2 m s E g m' E' g' cs lrs /=.
+  case Hmke1 : (mk_env_exp m s E g e1) => [[[[m1 E1] g1] cs1] ls1].
+  case Hmke2 : (mk_env_exp m1 s E1 g1 e2) => [[[[m2 E2] g2] cs2] ls2].
+  case Hmkr : (mk_env_xor E2 g2 ls1 ls2) => [[[Er gr] csr] lsr].
+  case=> _ _ <- <- _ Hgm Hgt.
+  rewrite !newer_than_cnf_append.
+  (* newer_than_cnf gr cs1 *)
+  move: (IH1 _ _ _ _ _ _ _ _ _ Hmke1 Hgm Hgt) => Hg1c1.
+  move: (mk_env_exp_newer_gen Hmke2) => Hg1g2.
+  move: (mk_env_xor_newer_gen Hmkr) => Hg2gr.
+  move: (newer_than_cnf_le_newer Hg1c1 (pos_leb_trans Hg1g2 Hg2gr)) => Hgrc1.
+  rewrite Hgrc1 /=.
+  (* newer_than_cnf gr cs2 *)
+  move: (mk_env_exp_newer_vm Hmke1 Hgm) => Hg1m1.
+  move: (mk_env_exp_newer_gen Hmke1) => Hgg1.
+  move: (newer_than_lit_le_newer Hgt Hgg1) => Hg1t.
+  move: (IH2 _ _ _ _ _ _ _ _ _ Hmke2 Hg1m1 Hg1t) => Hg2c2.
+  move: (newer_than_cnf_le_newer Hg2c2 Hg2gr) => Hgrc2.
+  rewrite Hgrc2 /=.
+  (* newer_than_cnf gr csr *)
+  move: (mk_env_exp_newer_res Hmke1 Hgm Hgt) => Hg1l1.
+  move: (mk_env_exp_newer_res Hmke2 Hg1m1 Hg1t) => Hg2l2.
+  move: (newer_than_lits_le_newer Hg1l1 Hg1g2) => Hg2l1.
+  exact: (mk_env_xor_newer_cnf Hmkr Hg2l1 Hg2l2). 
+Qed.
 
 Lemma mk_env_exp_newer_cnf_neg :
   forall (w0 : nat) (e : QFBV64.exp w0) (m : vm) (s : QFBV64.State.t)
@@ -8531,7 +9013,9 @@ Proof.
   - move=> w e0 e1.
     move: (mk_env_exp_newer_cnf _ e0) (mk_env_exp_newer_cnf _ e1) => IHe0 IHe1.
     exact: (mk_env_exp_newer_cnf_or IHe0 IHe1).
-  - exact: mk_env_exp_newer_cnf_xor.
+  - move=> w e1 e2.
+    move: (mk_env_exp_newer_cnf _ e1) (mk_env_exp_newer_cnf _ e2) => IH1 IH2.
+    exact: (mk_env_exp_newer_cnf_xor IH1 IH2).
   - exact: mk_env_exp_newer_cnf_neg.
   - exact: mk_env_exp_newer_cnf_add.
   - exact: mk_env_exp_newer_cnf_sub.
@@ -8694,13 +9178,36 @@ Proof.
 Qed .  
 
 Lemma mk_env_exp_consistent_xor :
-  forall (w0 : nat) (e e0 : QFBV64.exp w0) (m : vm) (s : QFBV64.State.t)
-         (E : env) (g : generator) (m' : vm) (E' : env) (g' : generator)
-         (cs : cnf) (lrs : w0.-tuple literal),
-    mk_env_exp m s E g (QFBV64.bvXor w0 e e0) = (m', E', g', cs, lrs) ->
-    newer_than_vm g m -> consistent m E s -> consistent m' E' s.
+  forall (w : nat) (e1 : QFBV64.exp w),
+    (forall (m : vm) (s : QFBV64.State.t) (E : env) (g : generator)
+            (m' : vm) (E' : env) (g' : generator) (cs : cnf)
+            (lrs : w.-tuple literal),
+        mk_env_exp m s E g e1 = (m', E', g', cs, lrs) ->
+        newer_than_vm g m -> consistent m E s -> consistent m' E' s) ->
+    forall (e2 : QFBV64.exp w),
+      (forall (m : vm) (s : QFBV64.State.t) (E : env) (g : generator)
+              (m' : vm) (E' : env) (g' : generator) (cs : cnf)
+              (lrs : w.-tuple literal),
+          mk_env_exp m s E g e2 = (m', E', g', cs, lrs) ->
+          newer_than_vm g m -> consistent m E s -> consistent m' E' s) ->
+      forall (m : vm) (s : QFBV64.State.t) (E : env) (g : generator)
+             (m' : vm) (E' : env) (g' : generator) (cs : cnf) 
+             (lrs : w.-tuple literal),
+        mk_env_exp m s E g (QFBV64.bvXor w e1 e2) = (m', E', g', cs, lrs) ->
+        newer_than_vm g m -> consistent m E s -> consistent m' E' s.
 Proof.
-Admitted.
+  move=> w e1 IH1 e2 IH2 m s E g m' E' g' cs lrs /=.
+  case Hmke1 : (mk_env_exp m s E g e1) => [[[[m1 E1] g1] cs1] ls1].
+  case Hmke2 : (mk_env_exp m1 s E1 g1 e2) => [[[[m2 E2] g2] cs2] ls2].
+  case Hmkr : (mk_env_xor E2 g2 ls1 ls2) => [[[Er gr] csr] lsr].
+  case=> <- <- _ _ _ Hgm HcmE.
+  move: (IH1 _ _ _ _ _ _ _ _ _ Hmke1 Hgm HcmE) => Hcm1E1.
+  move: (mk_env_exp_newer_vm Hmke1 Hgm) => Hg1m1.
+  move: (IH2 _ _ _ _ _ _ _ _ _ Hmke2 Hg1m1 Hcm1E1) => Hcm2E2.
+  move: (mk_env_xor_preserve Hmkr) => HpE2Er.
+  move: (mk_env_exp_newer_vm Hmke2 Hg1m1) => Hg2m2.
+  exact: (env_preserve_consistent Hg2m2 HpE2Er Hcm2E2).
+Qed.
 
 Lemma mk_env_exp_consistent_neg :
   forall (w0 : nat) (e : QFBV64.exp w0) (m : vm) (s : QFBV64.State.t)
@@ -9191,7 +9698,9 @@ Proof.
   - move=> w e0 e1 .
     move: (mk_env_exp_consistent _ e0) (mk_env_exp_consistent _ e1) => IHe0 IHe1 .
     exact: (mk_env_exp_consistent_or IHe0 IHe1) .
-  - exact: mk_env_exp_consistent_xor.
+  - move=> w e1 e2.
+    move: (mk_env_exp_consistent _ e1) (mk_env_exp_consistent _ e2) => IH1 IH2.
+    exact: (mk_env_exp_consistent_xor IH1 IH2).
   - exact: mk_env_exp_consistent_neg.
   - exact: mk_env_exp_consistent_add.
   - exact: mk_env_exp_consistent_sub.
@@ -9345,13 +9854,36 @@ Proof.
 Qed .           
 
 Lemma mk_env_exp_preserve_xor :
-  forall (w0 : nat) (e e0 : QFBV64.exp w0) (m : vm) (s : QFBV64.State.t)
-         (E : env) (g : generator) (m' : vm) (E' : env) (g' : generator)
-         (cs : cnf) (lrs : w0.-tuple literal),
-    mk_env_exp m s E g (QFBV64.bvXor w0 e e0) = (m', E', g', cs, lrs) ->
-    env_preserve E E' g.
+  forall (w : nat) (e1 : QFBV64.exp w),
+    (forall (m : vm) (s : QFBV64.State.t) (E : env) (g : generator)
+            (m' : vm) (E' : env) (g' : generator) (cs : cnf)
+            (lrs : w.-tuple literal),
+        mk_env_exp m s E g e1 = (m', E', g', cs, lrs) -> env_preserve E E' g) ->
+    forall (e2 : QFBV64.exp w),
+      (forall (m : vm) (s : QFBV64.State.t) (E : env) (g : generator)
+              (m' : vm) (E' : env) (g' : generator) (cs : cnf)
+              (lrs : w.-tuple literal),
+          mk_env_exp m s E g e2 = (m', E', g', cs, lrs) -> env_preserve E E' g) ->
+      forall (m : vm) (s : QFBV64.State.t) (E : env) (g : generator)
+             (m' : vm) (E' : env) (g' : generator) (cs : cnf) 
+             (lrs : w.-tuple literal),
+        mk_env_exp m s E g (QFBV64.bvXor w e1 e2) = (m', E', g', cs, lrs) ->
+        env_preserve E E' g.
 Proof.
-Admitted.
+  move=> w e1 IH1 e2 IH2 m s E g m' E' g' cs lrs /=.
+  case Hmke1 : (mk_env_exp m s E g e1) => [[[[m1 E1] g1] cs1] ls1].
+  case Hmke2 : (mk_env_exp m1 s E1 g1 e2) => [[[[m2 E2] g2] cs2] ls2].
+  case Hmkr : (mk_env_xor E2 g2 ls1 ls2) => [[[Er gr] csr] lsr].
+  case=> _ <- _ _ _.
+  move: (IH1 _ _ _ _ _ _ _ _ _ Hmke1) => HpEE1g.
+  move: (IH2 _ _ _ _ _ _ _ _ _ Hmke2) => HpE1E2g1.
+  move: (mk_env_xor_preserve Hmkr) => HpE2Erg2.
+  move: (mk_env_exp_newer_gen Hmke1) (mk_env_exp_newer_gen Hmke2) => Hgg1 Hg1g2.
+  move: (env_preserve_le HpE1E2g1 Hgg1) => HpE1E2g.
+  move: (env_preserve_le HpE2Erg2 (pos_leb_trans Hgg1 Hg1g2)) => HpE2Erg.
+  apply: (env_preserve_trans _ HpE2Erg).
+  exact: (env_preserve_trans HpEE1g HpE1E2g).
+Qed.
 
 Lemma mk_env_exp_preserve_neg :
   forall (w0 : nat) (e : QFBV64.exp w0) (m : vm) (s : QFBV64.State.t)
@@ -9833,7 +10365,9 @@ Proof.
   - move => w e0 e1 .
     move: (mk_env_exp_preserve _ e0) (mk_env_exp_preserve _ e1) => IHe0 IHe1 .
     exact: (mk_env_exp_preserve_or IHe0 IHe1) .
-  - exact: mk_env_exp_preserve_xor.
+  - move=> w e1 e2.
+    move: (mk_env_exp_preserve _ e1) (mk_env_exp_preserve _ e2) => IH1 IH2.
+    exact: (mk_env_exp_preserve_xor IH1 IH2).
   - exact: mk_env_exp_preserve_neg.
   - exact: mk_env_exp_preserve_add.
   - exact: mk_env_exp_preserve_sub.
@@ -10030,15 +10564,51 @@ Proof.
 Qed.   
 
 Lemma mk_env_exp_sat_xor :
-  forall (w0 : nat) (e e0 : QFBV64.exp w0) (m : vm) (s : QFBV64.State.t)
-         (E : env) (g : generator) (m' : vm) (E' : env) (g' : generator)
-         (cs : cnf) (lrs : w0.-tuple literal),
-    mk_env_exp m s E g (QFBV64.bvXor w0 e e0) = (m', E', g', cs, lrs) ->
-    newer_than_vm g m ->
-    newer_than_lit g lit_tt ->
-    interp_cnf E' cs.
+  forall (w : nat) (e1 : QFBV64.exp w),
+    (forall (m : vm) (s : QFBV64.State.t) (E : env) (g : generator)
+            (m' : vm) (E' : env) (g' : generator) (cs : cnf)
+            (lrs : w.-tuple literal),
+        mk_env_exp m s E g e1 = (m', E', g', cs, lrs) ->
+        newer_than_vm g m -> newer_than_lit g lit_tt -> interp_cnf E' cs) ->
+    forall (e2 : QFBV64.exp w),
+      (forall (m : vm) (s : QFBV64.State.t) (E : env) (g : generator)
+              (m' : vm) (E' : env) (g' : generator) (cs : cnf)
+              (lrs : w.-tuple literal),
+          mk_env_exp m s E g e2 = (m', E', g', cs, lrs) ->
+          newer_than_vm g m -> newer_than_lit g lit_tt -> interp_cnf E' cs) ->
+      forall (m : vm) (s : QFBV64.State.t) (E : env) (g : generator)
+             (m' : vm) (E' : env) (g' : generator) (cs : cnf) 
+             (lrs : w.-tuple literal),
+        mk_env_exp m s E g (QFBV64.bvXor w e1 e2) = (m', E', g', cs, lrs) ->
+        newer_than_vm g m -> newer_than_lit g lit_tt -> interp_cnf E' cs.
 Proof.
-Admitted.
+  move=> w e1 IH1 e2 IH2 m s E g m' E' g' cs lrs /=.
+  case Hmke1 : (mk_env_exp m s E g e1) => [[[[m1 E1] g1] cs1] ls1].
+  case Hmke2 : (mk_env_exp m1 s E1 g1 e2) => [[[[m2 E2] g2] cs2] ls2].
+  case Hmkr : (mk_env_xor E2 g2 ls1 ls2) => [[[Er gr] csr] lsr].
+  case=> _ <- _ <- _ Hgm Hgt. rewrite !interp_cnf_append.
+  (* interp_cnf Er cs1 *)
+  move: (IH1 _ _ _ _ _ _ _ _ _ Hmke1 Hgm Hgt) => HiE1c1.
+  move: (mk_env_exp_preserve Hmke2) => HpE1E2g1.
+  move: (mk_env_xor_preserve Hmkr) => HpE2Erg2.
+  move: (mk_env_exp_newer_gen Hmke2) => Hg1g2.
+  move: (env_preserve_le HpE2Erg2 Hg1g2) => HpE2Erg1.
+  move: (env_preserve_trans HpE1E2g1 HpE2Erg1) => HpE1Erg1.
+  move: (mk_env_exp_newer_cnf Hmke1 Hgm Hgt) => Hg1c1.
+  rewrite (env_preserve_cnf HpE1Erg1 Hg1c1) HiE1c1 /=.
+  (* interp_cnf Er cs2 *)
+  move: (mk_env_exp_newer_vm Hmke1 Hgm) => Hg1m1.
+  move: (mk_env_exp_newer_gen Hmke1) => Hgg1.
+  move: (newer_than_lit_le_newer Hgt Hgg1) => Hg1t.
+  move: (IH2 _ _ _ _ _ _ _ _ _ Hmke2 Hg1m1 Hg1t) => HiE2c2.
+  move: (mk_env_exp_newer_cnf Hmke2 Hg1m1 Hg1t) => Hg2c2.
+  rewrite (env_preserve_cnf HpE2Erg2 Hg2c2) HiE2c2 /=.
+  (* interp_cnf Er csr *)
+  move: (mk_env_exp_newer_res Hmke1 Hgm Hgt) => Hg1l1.
+  move: (mk_env_exp_newer_res Hmke2 Hg1m1 Hg1t) => Hg2l2.
+  move: (newer_than_lits_le_newer Hg1l1 Hg1g2) => Hg2l1.
+  exact: (mk_env_xor_sat Hmkr Hg2l1 Hg2l2).
+Qed.
 
 Lemma mk_env_exp_sat_neg :
   forall (w0 : nat) (e : QFBV64.exp w0) (m : vm) (s : QFBV64.State.t)
@@ -10663,7 +11233,9 @@ Proof.
   - move=> w e0 e1 .
     move: (mk_env_exp_sat _ e0) (mk_env_exp_sat _ e1) => IHe0 IHe1 .
     exact: (mk_env_exp_sat_or IHe0 IHe1) .
-  - exact: mk_env_exp_sat_xor.
+  - move=> w e1 e2.
+    move: (mk_env_exp_sat _ e1) (mk_env_exp_sat _ e2) => IH1 IH2.
+    exact: (mk_env_exp_sat_xor IH1 IH2).
   - exact: mk_env_exp_sat_neg.
   - exact: mk_env_exp_sat_add.
   - exact: mk_env_exp_sat_sub.
